PulseHashTable: pht becomes erased argument. Array: use BoundedIntegers class

pulse/share/steel/examples/pulse/lib/PulseHashTable.fst
@@ -24,19 +24,40 @@ type pht_sig_us = {
   valt : Type0;
   hashf : keyt -> US.t;
 }
+let mk_pht_sig_us keyt valt hashf : pht_sig_us = { keyt; valt; hashf }
 
 noeq
 type ht_t (s : pht_sig_us) = {
   sz : pos_us;
   contents : A.larray (cell s.keyt s.valt) (US.v sz);
 }
+let mk_ht (#s:pht_sig_us) (sz:pos_us) 
+          (contents:A.larray (cell s.keyt s.valt) (US.v sz))
+  : ht_t s 
+  = { sz; contents; }
 
 let s_to_ps (s:pht_sig_us) : pht_sig
   = { keyt = s.keyt; valt = s.valt; hashf = (fun k -> US.v (s.hashf k)) }
 
+let mk_init_pht (#s:pht_sig_us) (sz:pos_us)
+  : pht_t (s_to_ps s)
+  = 
+  { sz = US.v sz;
+    spec = (fun (k:s.keyt) -> None);
+    repr = Seq.create (US.v sz) Clean;
+    inv = (); }
+
 let models (s:pht_sig_us) (ht:ht_t s) (pht:pht_t (s_to_ps s)) : vprop
 = A.pts_to ht.contents full_perm pht.repr `star`
-  pure (US.v ht.sz == pht.sz)
+  pure (
+    US.v ht.sz == pht.sz /\
+    A.is_full_array ht.contents
+  )
+
+let ht_perm (s:pht_sig_us) (ht: ht_t s) : vprop
+  = exists_ (fun (pht:pht_t (s_to_ps s)) -> models s ht pht) // FIXME: this is erasing the pht
+
+type locked_ht_t (s:pht_sig_us) = ht:ht_t s & LK.lock (ht_perm s ht)
 
 let canonical_index_us (#s:pht_sig_us) (k:s.keyt) (sz:pos_us) 
   : US.t = s.hashf k % sz
@@ -45,9 +66,11 @@ let modulo_us (v1 v2:US.t) (m:pos_us) (_:squash(US.fits (US.v v1 + US.v v2)))
   : US.t 
   = (v1 + v2) % m
 
+let pht_sz #s (pht:pht_t s) : pos = pht.sz
+
 ```pulse
 fn pulse_lookup_index (#s:pht_sig_us)
-                      (#pht:(p:pht_t (s_to_ps s){not_full p.repr}))  
+                      (#pht:erased (pht_t (s_to_ps s)))
                       (ht:ht_t s) (k:s.keyt)
   requires models s ht pht
   returns  o:(o:option (s.valt & US.t){o == PHT.lookup_index_us pht k})
@@ -67,10 +90,10 @@ fn pulse_lookup_index (#s:pht_sig_us)
     R.pts_to cont full_perm vcont **
     R.pts_to ret full_perm (if vcont then None else (PHT.lookup_index_us pht k)) **
     pure (
-      US.v ht.sz == pht.sz /\
+      US.v ht.sz == pht_sz pht /\
       voff <= ht.sz /\
-      walk_get_idx #(s_to_ps s) #pht.sz pht.repr (US.v cidx) k (US.v voff) 
-        == lookup_repr_index #(s_to_ps s) #pht.sz pht.repr k /\
+      walk_get_idx #(s_to_ps s) #(pht_sz pht) pht.repr (US.v cidx) k (US.v voff) 
+        == lookup_repr_index #(s_to_ps s) #(pht_sz pht) pht.repr k /\
       b == (voff <= ht.sz && vcont = true)
     ))
   {
@@ -116,7 +139,7 @@ fn pulse_lookup_index (#s:pht_sig_us)
 
 ```pulse
 fn lookup (#s:pht_sig_us)
-          (#pht:(p:pht_t (s_to_ps s){not_full p.repr}))  
+          (#pht:erased (pht_t (s_to_ps s)))
           (ht:ht_t s) (k:s.keyt)
   requires models s ht pht
   returns  o:(o:option s.valt{o == PHT.lookup pht k})
@@ -132,7 +155,7 @@ fn lookup (#s:pht_sig_us)
 
 ```pulse
 fn insert (#s:pht_sig_us)
-          (#pht:(p:pht_t (s_to_ps s){not_full p.repr})) 
+          (#pht:(p:erased (pht_t (s_to_ps s)){not_full p.repr}))
           (ht:ht_t s) (k:s.keyt) (v:s.valt)
   requires models s ht pht
   ensures  models s ht (PHT.insert pht k v)
@@ -149,12 +172,12 @@ fn insert (#s:pht_sig_us)
     R.pts_to cont full_perm vcont **
     A.pts_to ht.contents full_perm (if vcont then pht.repr else (PHT.insert pht k v).repr) **
     pure (
-      US.v ht.sz == pht.sz /\
+      US.v ht.sz == pht_sz pht /\
       voff <= ht.sz /\
       strong_all_used_not_by pht.repr (US.v cidx) (US.v voff) k /\
       walk pht.repr (US.v cidx) k (US.v voff) == lookup_repr pht.repr k /\
-      insert_repr_walk #(s_to_ps s) #pht.sz #pht.spec pht.repr k v (US.v voff) (US.v cidx) () () 
-        == insert_repr #(s_to_ps s) #pht.sz #pht.spec pht.repr k v /\
+      insert_repr_walk #(s_to_ps s) #(pht_sz pht) #pht.spec pht.repr k v (US.v voff) (US.v cidx) () () 
+        == insert_repr #(s_to_ps s) #(pht_sz pht) #pht.spec pht.repr k v /\
       b == (voff <= ht.sz && vcont = true)
     ))
   {
@@ -171,7 +194,7 @@ fn insert (#s:pht_sig_us)
           if (k' = k) {
             op_Array_Assignment ht.contents idx (mk_used_cell k v);
             cont := false;
-            assert (pure (insert_repr #(s_to_ps s) #pht.sz #pht.spec pht.repr k v `Seq.equal` 
+            assert (pure (insert_repr #(s_to_ps s) #(pht_sz pht) #pht.spec pht.repr k v `Seq.equal` 
               Seq.upd pht.repr (US.v idx) (mk_used_cell k v))); 
           } else {
             off := voff + 1sz;
@@ -180,7 +203,7 @@ fn insert (#s:pht_sig_us)
         Clean -> {
           op_Array_Assignment ht.contents idx (mk_used_cell k v);
           cont := false;
-          assert (pure (insert_repr #(s_to_ps s) #pht.sz #pht.spec pht.repr k v `Seq.equal` 
+          assert (pure (insert_repr #(s_to_ps s) #(pht_sz pht) #pht.spec pht.repr k v `Seq.equal` 
             Seq.upd pht.repr (US.v idx) (mk_used_cell k v)));
         }
         Zombie -> {
@@ -192,13 +215,13 @@ fn insert (#s:pht_sig_us)
               op_Array_Assignment ht.contents (snd p) Zombie;
               op_Array_Assignment ht.contents idx (mk_used_cell k v);
               cont := false;
-              assert (pure (insert_repr #(s_to_ps s) #pht.sz #pht.spec pht.repr k v `Seq.equal` 
+              assert (pure (insert_repr #(s_to_ps s) #(pht_sz pht) #pht.spec pht.repr k v `Seq.equal` 
                 Seq.upd (Seq.upd pht.repr (US.v (snd p)) Zombie) (US.v idx) (mk_used_cell k v)));
             }
             None -> { 
               op_Array_Assignment ht.contents idx (mk_used_cell k v); 
               cont := false;
-              assert (pure (insert_repr #(s_to_ps s) #pht.sz #pht.spec pht.repr k v 
+              assert (pure (insert_repr #(s_to_ps s) #(pht_sz pht) #pht.spec pht.repr k v 
                 `Seq.equal` Seq.upd pht.repr (US.v idx) (mk_used_cell k v)));
             }
           };
@@ -212,7 +235,7 @@ fn insert (#s:pht_sig_us)
 
 ```pulse
 fn delete (#s:pht_sig_us)
-          (#pht:pht_t (s_to_ps s)) 
+          (#pht:erased (pht_t (s_to_ps s)))
           (ht:ht_t s) (k:s.keyt)
   requires models s ht pht
   ensures  models s ht (PHT.delete pht k)
@@ -229,12 +252,12 @@ fn delete (#s:pht_sig_us)
     R.pts_to cont full_perm vcont **
     A.pts_to ht.contents full_perm (if vcont then pht.repr else (PHT.delete pht k).repr) **
     pure (
-      US.v ht.sz == pht.sz /\
+      US.v ht.sz == pht_sz pht /\
       voff <= ht.sz /\
       all_used_not_by pht.repr (US.v cidx) (US.v voff) k /\
       walk pht.repr (US.v cidx) k (US.v voff) == lookup_repr pht.repr k /\
-      delete_repr_walk #(s_to_ps s) #pht.sz #pht.spec pht.repr k (US.v voff) (US.v cidx) () () 
-        == delete_repr #(s_to_ps s) #pht.sz #pht.spec pht.repr k /\
+      delete_repr_walk #(s_to_ps s) #(pht_sz pht) #pht.spec pht.repr k (US.v voff) (US.v cidx) () () 
+        == delete_repr #(s_to_ps s) #(pht_sz pht) #pht.spec pht.repr k /\
       b == (voff <= ht.sz && vcont = true)
     ))
   {
